src/hls/Veriloggenproof.v
@@ -225,6 +225,116 @@ Proof.
 Qed.
 Hint Resolve mis_stepp_decl : verilogproof.
 
+Lemma mis_stepp_negedge_decl :
+  forall l asr asa f,
+    mis_stepp_negedge f asr asa (map Vdeclaration l) asr asa.
+Proof.
+  induction l.
+  - intros. constructor.
+  - intros. simplify. econstructor. constructor. auto.
+Qed.
+Hint Resolve mis_stepp_negedge_decl : verilogproof.
+
+Lemma mod_entrypoint_equiv m : mod_entrypoint (transl_module m) = HTL.mod_entrypoint m.
+Proof. unfold transl_module; intros; destruct (HTL.mod_ram m) eqn:?; crush. Qed.
+
+Lemma mod_st_equiv m : mod_st (transl_module m) = HTL.mod_st m.
+Proof. unfold transl_module; intros; destruct (HTL.mod_ram m) eqn:?; crush. Qed.
+
+Lemma mod_stk_equiv m : mod_stk (transl_module m) = HTL.mod_stk m.
+Proof. unfold transl_module; intros; destruct (HTL.mod_ram m) eqn:?; crush. Qed.
+
+Lemma mod_stk_len_equiv m : mod_stk_len (transl_module m) = HTL.mod_stk_len m.
+Proof. unfold transl_module; intros; destruct (HTL.mod_ram m) eqn:?; crush. Qed.
+
+Lemma mod_finish_equiv m : mod_finish (transl_module m) = HTL.mod_finish m.
+Proof. unfold transl_module; intros; destruct (HTL.mod_ram m) eqn:?; crush. Qed.
+
+Lemma mod_reset_equiv m : mod_reset (transl_module m) = HTL.mod_reset m.
+Proof. unfold transl_module; intros; destruct (HTL.mod_ram m) eqn:?; crush. Qed.
+
+Lemma mod_clk_equiv m : mod_clk (transl_module m) = HTL.mod_clk m.
+Proof. unfold transl_module; intros; destruct (HTL.mod_ram m) eqn:?; crush. Qed.
+
+Lemma mod_return_equiv m : mod_return (transl_module m) = HTL.mod_return m.
+Proof. unfold transl_module; intros; destruct (HTL.mod_ram m) eqn:?; crush. Qed.
+
+Lemma mod_params_equiv m : mod_args (transl_module m) = HTL.mod_params m.
+Proof. unfold transl_module; intros; destruct (HTL.mod_ram m) eqn:?; crush. Qed.
+
+Lemma empty_stack_equiv m : empty_stack (transl_module m) = HTL.empty_stack m.
+Proof. unfold transl_module; intros; destruct (HTL.mod_ram m) eqn:?; crush. Qed.
+
+Ltac rewrite_eq := rewrite mod_return_equiv
+                   || rewrite mod_clk_equiv
+                   || rewrite mod_reset_equiv
+                   || rewrite mod_finish_equiv
+                   || rewrite mod_stk_len_equiv
+                   || rewrite mod_stk_equiv
+                   || rewrite mod_st_equiv
+                   || rewrite mod_entrypoint_equiv
+                   || rewrite mod_params_equiv
+                   || rewrite empty_stack_equiv.
+
+Lemma find_assocmap_get r i v : r ! i = Some v -> r # i = v.
+Proof.
+  intros. unfold find_assocmap, AssocMapExt.get_default. rewrite H. auto.
+Qed.
+
+Lemma ram_exec_match :
+  forall f asr asa asr' asa' r clk,
+    HTL.exec_ram asr asa (Some r) asr' asa' ->
+    mi_stepp_negedge f asr asa (inst_ram clk r) asr' asa'.
+Proof.
+  inversion 1; subst; simplify.
+  { unfold inst_ram. econstructor.
+    eapply stmnt_runp_Vcond_false.
+    econstructor. econstructor. econstructor. auto.
+    econstructor. auto.
+    simplify.
+    unfold boolToValue, natToValue, valueToBool.
+    rewrite Int.eq_sym. rewrite H3. simplify.
+    auto. constructor. }
+  { unfold inst_ram. econstructor. econstructor. econstructor.
+    econstructor. econstructor. auto.
+    econstructor. auto.
+    simplify.
+    unfold boolToValue, natToValue, valueToBool.
+    pose proof H4 as X. apply find_assocmap_get in X.
+    rewrite X. rewrite Int.eq_sym. rewrite H1. auto.
+    econstructor. econstructor. econstructor. econstructor.
+    pose proof H5 as X. apply find_assocmap_get in X.
+    rewrite X.
+    unfold valueToBool. unfold ZToValue in *.
+    unfold Int.eq in H2.
+    unfold uvalueToZ.
+    assert (Int.unsigned wr_en =? 0 = false).
+    apply Z.eqb_neq. rewrite Int.unsigned_repr in H2 by (simplify; lia).
+    destruct (zeq (Int.unsigned wr_en) 0); crush.
+    rewrite H0. auto.
+    apply stmnt_runp_Vnonblock_arr. econstructor. econstructor. auto.
+    econstructor. econstructor.
+    apply find_assocmap_get in H9. rewrite H9.
+    apply find_assocmap_get in H6. rewrite H6.
+    repeat econstructor. apply find_assocmap_get; auto.
+  }
+  { econstructor. econstructor. econstructor. econstructor. auto.
+    econstructor. auto.
+    econstructor.
+    unfold boolToValue, natToValue, valueToBool.
+    apply find_assocmap_get in H3. rewrite H3.
+    rewrite Int.eq_sym. rewrite H1. auto.
+    econstructor.
+    eapply stmnt_runp_Vcond_false. econstructor. auto.
+    simplify. apply find_assocmap_get in H4. rewrite H4.
+    auto.
+    repeat (econstructor; auto). apply find_assocmap_get in H5.
+    rewrite H5. eassumption.
+    repeat econstructor. simplify. apply find_assocmap_get; auto.
+  }
+Qed.
+
+
 Section CORRECTNESS.
 
   Variable prog: HTL.program.
@@ -269,6 +379,12 @@ Section CORRECTNESS.
   Qed.
   Hint Resolve senv_preserved : verilogproof.
 
+  Ltac unfold_replace :=
+    match goal with
+    | H: HTL.mod_ram _ = _ |- context[transl_module] =>
+      unfold transl_module; rewrite H
+    end.
+
   Theorem transl_step_correct :
     forall (S1 : HTL.state) t S2,
       HTL.step ge S1 t S2 ->
@@ -276,13 +392,61 @@ Section CORRECTNESS.
         match_states S1 R1 ->
         exists R2, Smallstep.plus step tge R1 t R2 /\ match_states S2 R2.
   Proof.
-    induction 1; intros R1 MSTATE; inv MSTATE.
-    Admitted.
-(*    - econstructor; split. apply Smallstep.plus_one. econstructor.
-      assumption. assumption. eassumption. apply valueToPos_posToValue.
+    induction 1; intros R1 MSTATE; inv MSTATE; destruct (HTL.mod_ram m) eqn:?.
+    - econstructor; split. apply Smallstep.plus_one. econstructor.
+      unfold_replace. assumption. unfold_replace. assumption.
+      unfold_replace. eassumption. apply valueToPos_posToValue.
       split. lia.
       eapply pc_wf. intros. pose proof (HTL.mod_wf m) as HP. destruct HP as [HP _].
       split. lia. apply HP. eassumption. eassumption.
+      unfold_replace.
+      econstructor. econstructor. eapply stmnt_runp_Vcond_false. econstructor. econstructor.
+      simpl. unfold find_assocmap. unfold AssocMapExt.get_default.
+      rewrite H. trivial.
+
+      econstructor. simpl. auto. auto.
+
+      eapply transl_list_correct.
+      intros. split. lia. pose proof (HTL.mod_wf m) as HP. destruct HP as [HP _]. auto.
+      apply Maps.PTree.elements_keys_norepet. eassumption.
+      2: { apply valueToPos_inj. apply unsigned_posToValue_le.
+           eapply pc_wf. intros. pose proof (HTL.mod_wf m) as HP. destruct HP as [HP _].
+           split. lia. apply HP. eassumption. eassumption.
+           apply unsigned_posToValue_le. eapply pc_wf. intros. pose proof (HTL.mod_wf m) as HP.
+           destruct HP as [HP _].
+           split. lia. apply HP. eassumption. eassumption. trivial.
+      }
+      apply Maps.PTree.elements_correct. eassumption. eassumption.
+
+      econstructor. econstructor.
+
+      eapply transl_list_correct.
+      intros. split. lia. pose proof (HTL.mod_wf m) as HP. destruct HP as [_ HP]. auto.
+      apply Maps.PTree.elements_keys_norepet. eassumption.
+      2: { apply valueToPos_inj. apply unsigned_posToValue_le.
+           eapply pc_wf. intros. pose proof (HTL.mod_wf m) as HP. destruct HP as [HP _].
+           split. lia. apply HP. eassumption. eassumption.
+           apply unsigned_posToValue_le. eapply pc_wf. intros. pose proof (HTL.mod_wf m) as HP.
+           destruct HP as [HP _].
+           split. lia. apply HP. eassumption. eassumption. trivial.
+      }
+      apply Maps.PTree.elements_correct. eassumption. eassumption.
+      econstructor. econstructor.
+      apply mis_stepp_decl. simplify. unfold_replace. simplify.
+      econstructor. econstructor. econstructor. econstructor.
+      econstructor.
+      apply ram_exec_match. eauto.
+      apply mis_stepp_negedge_decl. simplify. auto. auto.
+      rewrite_eq. eauto. auto.
+      rewrite valueToPos_posToValue. econstructor. auto.
+      simplify; lia.
+    - inv H7. econstructor; split. apply Smallstep.plus_one. econstructor.
+      unfold_replace. assumption. unfold_replace. assumption.
+      unfold_replace. eassumption. apply valueToPos_posToValue.
+      split. lia.
+      eapply pc_wf. intros. pose proof (HTL.mod_wf m) as HP. destruct HP as [HP _].
+      split. lia. apply HP. eassumption. eassumption.
+      unfold_replace.
       econstructor. econstructor. eapply stmnt_runp_Vcond_false. econstructor. econstructor.
       simpl. unfold find_assocmap. unfold AssocMapExt.get_default.
       rewrite H. trivial.
@@ -315,18 +479,28 @@ Section CORRECTNESS.
       }
       apply Maps.PTree.elements_correct. eassumption. eassumption.
 
-      apply mis_stepp_decl. trivial. trivial. simpl. eassumption. auto.
-      rewrite valueToPos_posToValue. constructor; assumption. lia.
-
-    - econstructor; split. apply Smallstep.plus_one. apply step_finish. assumption. eassumption.
+      apply mis_stepp_decl. simplify.
+      unfold_replace.
+      repeat econstructor. apply mis_stepp_negedge_decl. trivial. trivial.
+      simpl. unfold_replace. eassumption. auto. simplify.
+      rewrite valueToPos_posToValue. constructor; eassumption. simplify; lia.
+    - econstructor; split. apply Smallstep.plus_one. apply step_finish.
+      rewrite_eq. assumption.
+      rewrite_eq. eassumption.
+      econstructor; auto.
+    - econstructor; split. apply Smallstep.plus_one. apply step_finish.
+      unfold transl_module. rewrite Heqo. simplify.
+      assumption. unfold_replace. eassumption.
       constructor; assumption.
     - econstructor; split. apply Smallstep.plus_one. constructor.
-
-      constructor. constructor.
+      repeat rewrite_eq. constructor. constructor.
+    - econstructor; split. apply Smallstep.plus_one. constructor.
+      repeat rewrite_eq. constructor. constructor.
     - inv H3. econstructor; split. apply Smallstep.plus_one. constructor. trivial.
-
-      apply match_state. assumption.
-  Qed.*)
+      repeat rewrite_eq. apply match_state. assumption.
+    - inv H3. econstructor; split. apply Smallstep.plus_one. constructor. trivial.
+      repeat rewrite_eq. apply match_state. assumption.
+  Qed.
   Hint Resolve transl_step_correct : verilogproof.
 
   Lemma transl_initial_states :
